aaaaaand one logical relation!

code/theories/Bidir.v
@@ -1,66 +1,66 @@
 From Interpolation Require Import Utils Syntax Notations Typing.
 From Stdlib Require Import Relations Arith Lia Bool List.
 
-Reserved Notation "Γ '|-' t ▹ T"
+Reserved Notation "Γ '⊢' t ▹ T"
   (at level 101, t at level 59).
-Reserved Notation "Γ '|-' t ◃ T"
+Reserved Notation "Γ '⊢' t ◃ T"
   (at level 101, t at level 59).
 
 Unset Elimination Schemes.
 
 Inductive normal : context -> type -> term -> Prop :=
-| C_Star Γ : (Γ |- tStar ◃ TUnit)
+| C_Star Γ : (Γ ⊢ tStar ◃ TUnit)
 
 | C_Abs Γ (A B : type) t :
-  (Γ ,, A |- t ◃ B) ->
-  Γ |- tLam t ◃ TFun A B
+  (Γ ,, A ⊢ t ◃ B) ->
+  Γ ⊢ tLam t ◃ TFun A B
 
 | C_Pair Γ A B a b :
-  (Γ |- a ◃ A) ->
-  (Γ |- b ◃ B) ->
-  (Γ |- tPair a b ◃ TProd A B)
+  (Γ ⊢ a ◃ A) ->
+  (Γ ⊢ b ◃ B) ->
+  (Γ ⊢ tPair a b ◃ TProd A B)
 
 | C_Left Γ A B a :
-  (Γ |- a ◃ A) ->
-  (Γ |- tLeft a ◃ TSum A B)
+  (Γ ⊢ a ◃ A) ->
+  (Γ ⊢ tLeft a ◃ TSum A B)
 
 | C_Right Γ A B b :
-  (Γ |- b ◃ B) ->
-  (Γ |- tRight b ◃ TSum A B)
+  (Γ ⊢ b ◃ B) ->
+  (Γ ⊢ tRight b ◃ TSum A B)
 
 | C_Abort Γ A t :
-  (Γ |- t ◃ TEmp) ->
-  (Γ |- tAbort t ◃ A)
+  (Γ ⊢ t ▹ TEmp) ->
+  (Γ ⊢ tAbort t ◃ A)
 
 | C_If Γ A B T s bl br :
-  (Γ |- s ▹ TSum A B) ->
-  (Γ,,A |- bl ◃ T) ->
-  (Γ,,B |- br ◃ T) ->
-  (Γ |- tIf s bl br ◃ T)
+  (Γ ⊢ s ▹ TSum A B) ->
+  (Γ,,A ⊢ bl ◃ T) ->
+  (Γ,,B ⊢ br ◃ T) ->
+  (Γ ⊢ tIf s bl br ◃ T)
 
 | C_inf Γ A A' t :
-  (Γ |- t ▹ A') ->
+  (Γ ⊢ t ▹ A') ->
   A' = A ->
-  (Γ |- t ◃ A)
+  (Γ ⊢ t ◃ A)
 
 with neutral : context -> type -> term -> Prop :=
 | I_Var Γ n T :
   in_context n Γ T ->
-  Γ |- tVar n ▹ T
+  Γ ⊢ tVar n ▹ T
 
 | I_App Γ A B f u :
-  (Γ |- f ▹ TFun A B) ->
-  (Γ |- u ◃ A) ->
-  Γ |- tApp f u ▹ B
+  (Γ ⊢ f ▹ TFun A B) ->
+  (Γ ⊢ u ◃ A) ->
+  Γ ⊢ tApp f u ▹ B
 
 | I_Proj Γ A B (b : bool) t :
-  (Γ |- t ▹ TProd A B) ->
-  (Γ |- tProj b t ▹ (if b then A else B))
+  (Γ ⊢ t ▹ TProd A B) ->
+  (Γ ⊢ tProj b t ▹ (if b then A else B))
 
-where "Γ '|-' t ▹ T" := (neutral Γ T t) (Γ in scope context_scope)
-and "Γ '|-' t ◃ T" := (normal Γ T t) (Γ in scope context_scope).
+where "Γ '⊢' t ▹ T" := (neutral Γ T t) (Γ in scope context_scope)
+and "Γ '⊢' t ◃ T" := (normal Γ T t) (Γ in scope context_scope).
 
-Hint Constructors neutral normal : core.
+Hint Constructors neutral normal : typing.
 
 Scheme 
 Minimality for normal Sort Prop with
@@ -77,7 +77,7 @@ exact t').
 Arguments bidir_concl Pnf Pne : rename.
 
 
-Theorem bidir_typing : bidir_concl (fun Γ T t => (Γ |- t :: T)) (fun Γ T t => (Γ |- t :: T)).
+Theorem bidir_typing : bidir_concl (fun Γ T t => (Γ ⊢ t :: T)) (fun Γ T t => (Γ ⊢ t :: T)).
 Proof.
   apply bidir_ind.
   all: try solve [now econstructor].
@@ -86,3 +86,28 @@ Proof.
     destruct b.
     all: now econstructor.
 Qed.
+
+Lemma ren_bidir : bidir_concl
+  (fun Γ T t => forall Δ ρ, (Δ ⊢ ρ :: Γ) -> Δ ⊢ t⟨ρ⟩ ◃ T)
+  (fun Γ T t => forall Δ ρ, (Δ ⊢ ρ :: Γ) -> Δ ⊢ t⟨ρ⟩ ▹ T).
+Proof.
+  apply bidir_ind ; eauto 10 with typing.
+Qed.
+
+Corollary ren_ne (Δ Γ : context) (T : type) (t : term) (r : ren) :
+  (Γ ⊢ t ▹ T) ->
+  (Δ ⊢ r :: Γ) ->
+  Δ ⊢ t⟨r⟩ ▹ T.
+Proof.
+  intros ; now eapply ren_bidir.
+Qed.
+
+Corollary ren_nf (Δ Γ : context) (T : type) (t : term) (r : ren) :
+  (Γ ⊢ t ◃ T) ->
+  (Δ ⊢ r :: Γ) ->
+  Δ ⊢ t⟨r⟩ ◃ T.
+Proof.
+  intros ; now eapply ren_bidir.
+Qed.
+
+Hint Resolve ren_ne ren_nf : typing.
