code/theories/MetaTheory.v
@@ -1,0 +1,734 @@
+From Interpolation Require Import Utils Syntax Notations Reduction Typing Bidir.
+From Stdlib Require Import Relations Arith Lia Bool List.
+
+(** ** Preservation of typing under reduction *)
+
+Lemma preservation_one (Γ : context) (T : type) (t u : term) : (Γ ⊢ t :: T) -> t ⤳ u -> (Γ ⊢ u :: T).
+Proof.
+  intros Hty Hred.
+  induction Hred in Γ, T, Hty |- *.
+  all: try (match goal with | e : elim |- _ => destruct e ; cbn in * end ; try solve [congruence]).
+  all: try (match goal with | e : _ = _ |- _ => inversion e ; subst end).
+  all: repeat match goal with | H : (_ ⊢ _ _ :: _) |- _ => inversion H ; subst ; clear H ; refold end.
+  all: eauto 20 with typing.
+Qed.
+
+Lemma preservation (Γ : context) (T : type) (t u : term) : (Γ ⊢ t :: T) -> t ⤳* u -> (Γ ⊢ u :: T).
+Proof.
+  induction 2 ; eauto using preservation_one.
+Qed.
+
+(** ** Progress *)
+(** A well-typed term is either a normal form, or can do a reduction step*)
+
+Lemma progress (Γ : context) (T : type) (t : term) :
+  (Γ ⊢ t :: T) -> (Γ ⊢ t ◃ T) \/ (exists u, t ⤳ u).
+Proof.
+  intros Hty.
+  induction Hty ; refold.
+  all: repeat match goal with
+    | IH : _ \/ _ |- _ => destruct IH as [?|[]] ; [|right ; eexists ; now econstructor] end.
+  all: try solve [left ; eauto with typing].
+  all: match goal with
+      | IH : _ ⊢ _ ◃ (_ _) |- _ => (inversion IH ; subst ; clear IH)
+      | IH : _ ⊢ _ ◃ TEmp |- _ => inversion IH ; subst ; clear IH
+    end ;
+    try solve [right ; eexists ; now constructor].
+  all: left ; eauto with typing.
+Qed.
+
+(** ** Bidirectional typing characterises well-typed normal forms *)
+
+Lemma bidir_normal_ind : bidir_concl
+  (fun Γ T t => forall u, t ⤳ u -> False)
+  (fun Γ T t => forall u, t ⤳ u -> False).
+Proof.
+  apply bidir_ind ; intros ; eauto.
+  all: match goal with H : _ ⤳ _ |- _ => inversion H ; subst ; refold ; clear H end ; eauto.
+  all: match goal with H : _ ⊢ _ ▹ _ |- _ => inversion H end.
+Qed.
+
+Lemma normal_bidir Γ T t :
+  (Γ ⊢ t ◃ T) <-> ((Γ ⊢ t :: T) /\ ~(exists u, t ⤳ u)).
+Proof.
+  split.
+  - intros Hty.
+    split.
+    + now apply bidir_typing in Hty.
+    + intros [? Hu].
+      now eapply bidir_normal_ind in Hty.
+  - intros [Hty ].
+    now apply progress in Hty as [|].
+Qed.
+
+
+
+
+
+(** ** Normalisation *)
+
+(** *** Covering *)
+(** A term is covered by a predicate if it is a case tree, with nodes eliminations of
+  neutrals of sum and empty types, and leaves terms that satisfy the predicate. *)
+Inductive covered (F : context -> term -> Prop) (Γ : context) : term -> Prop :=
+| cover_abort t : (Γ ⊢ t ▹ TEmp) -> covered F Γ (tAbort t)
+| cover_if A B s bl br :
+    (Γ ⊢ s ▹ TSum A B) ->
+    covered F (Γ,,A) bl -> covered F (Γ,,B) br ->
+    covered F Γ (tIf s bl br)
+| cover_ret t : F Γ t -> covered F Γ t.
+
+(** This forms a monad *)
+Definition map_cover F G Γ t : (forall Δ t, F Δ t -> G Δ t) -> covered F Γ t -> covered G Γ t.
+Proof.
+  intros f.
+  induction 1 ; now econstructor.
+Qed.
+
+Definition join_cover F Γ t : covered (covered F) Γ t -> covered F Γ t.
+Proof.
+  induction 1.
+  3: assumption.
+  all: now econstructor.
+Qed.
+
+(** And can be run on normal forms to yield a normal form *)
+Definition run_nf Γ T t : covered (fun Δ t => Δ ⊢ t ◃ T) Γ t -> Γ ⊢ t ◃ T.
+Proof.
+  induction 1 ; eauto with typing.
+Qed.
+
+(** *** Reducibility *)
+
+(** A term is reducible if it reduces to a value *)
+Definition _reducible (c : context -> type -> term -> Prop) (Γ : context) (T : type) (t : term) :=
+  exists t', t ⤳* t' /\ c Γ T t'.
+
+(**
+  A value at positive type is a cover of "proper values", which are either neutrals or constructors.
+  A value at negative type is a normal form that, when observed, yields reducible terms. *)
+
+Fixpoint value (Γ : context) (T : type) (t : term) : Prop :=
+  match T with
+  | TBase _ | TEmp => covered (fun Δ u => Δ ⊢ u ▹ T) Γ t
+  | TUnit => covered (fun Δ u => (Δ ⊢ u ▹ T) \/ u = tStar) Γ t
+  | TSum A B => covered
+    (fun Δ u => (Δ ⊢ u ▹ T) \/
+      (exists a, u = tLeft a /\ value Δ A a) \/ (exists b, u = tRight b /\ value Δ B b))
+    Γ t
+  | TProd A B => (Γ ⊢ t ◃ T) /\ (forall (b : bool), _reducible value Γ (if b then A else B) (tProj b t))
+  | TFun A B => (Γ ⊢ t ◃ T) /\
+      (forall Δ u ρ, (Δ ⊢ ρ :: Γ) -> _reducible value Δ A u -> _reducible value Δ B (tApp t⟨ρ⟩ u))
+  end.
+
+Notation reducible := (_reducible value).
+
+(** *** Semantic typing *)
+
+(** A reducible environment is one where all values are reducible *)
+Definition reducible_env (Δ Γ : context) (γ : subst) : Prop :=
+  forall i T, in_context i Γ T -> reducible Δ T (γ i).
+
+Instance sem_typing_env : HasSemTyping context context subst := reducible_env.
+
+(** A term is semantically well-typed if it yields reducible values in any reducible environment *)
+Definition sem_has_type (Γ : context) (T : type) (t : term) : Prop :=
+  forall (Δ : context) (γ : subst), (Δ ⊩ γ :: Γ) -> reducible Δ T t[γ].
+
+Instance sem_typing_term : HasSemTyping context type term := sem_has_type.
+
+Ltac fold_sem_typing :=
+  change sem_has_type with
+    (sem_typing (Ctx := context) (Ty := type) (Obj := term)) in * ;
+  change reducible_env with
+    (sem_typing (Ctx := context) (Ty := context) (Obj := subst)) in *.
+
+Smpl Add fold_sem_typing : refold.
+
+(** *** Easy lemmas on reducibility *)
+Lemma value_red Γ T t : value Γ T t -> reducible Γ T t.
+Proof.
+  intros.
+  eexists ; split ; eauto ; reflexivity.
+Qed. 
+
+Lemma red_antired {Γ T t} t' : reducible Γ T t' -> t ⤳* t' -> reducible Γ T t.
+Proof.
+  intros [v] ?.
+  exists v.
+  split ; [|easy].
+  now etransitivity.
+Qed.
+
+(** *** Reify/reflect *)
+(** Neutrals are always values, and values are always normal forms. *)
+
+Hint Extern 0 => (progress subst) : typing.
+
+Lemma reify_reflect (T : type) :
+  (forall Γ t, (Γ ⊢ t ▹ T) -> value Γ T t) /\ (forall Γ t, value Γ T t -> Γ ⊢ t ◃ T).
+Proof.
+  induction T ; cbn ; refold.
+  - split.
+    + intros.
+      now constructor.
+    + intros.
+      eapply run_nf, map_cover ; tea.
+      cbn ; eauto with typing.
+  - split.
+    + intros.
+      now constructor.
+    + intros.
+      eapply run_nf, map_cover ; tea.
+      cbn ; intuition eauto with typing. 
+  - split ; [|easy].
+    intros * Hne.
+    split ; [eauto with typing|].
+    intros b.
+    eexists ; split ; [reflexivity|..].
+    assert (Γ ⊢ tProj b t ▹ (if b then T1 else T2)) by now econstructor.
+    destruct b ; solve [now apply IHT1|now apply IHT2].
+  - split ; [|easy].
+    intros.
+    split.
+    1: now eauto with typing.
+    intros * ? [u' [Hred]].
+    apply (red_antired (tApp t⟨ρ⟩ u')).
+    2: now rewrite Hred.
+    eapply value_red, IHT2.
+    econstructor.
+    1: now eauto with typing.
+    now apply IHT1.
+  - split.
+    + intros.
+      now constructor.
+    + intros.
+      eapply run_nf, map_cover ; tea.
+      cbn ; eauto with typing.
+  - split.
+    + intros.
+      now constructor.
+    + intros.
+      eapply run_nf, map_cover ; tea.
+      intros * [|[[]|[]]].
+      all: cbn ; intuition eauto with typing.
+Qed.
+
+Corollary reflect Γ T t :  (Γ ⊢ t ▹ T) -> value Γ T t.
+Proof.
+  apply reify_reflect.
+Qed.
+
+Corollary reify Γ T t :  value Γ T t -> Γ ⊢ t ◃ T.
+Proof.
+  apply reify_reflect.
+Qed.
+
+(** *** Reducibility is stable under weakening *)
+
+Lemma ren_covered (F : context -> term -> Prop) (Δ Γ : context) (t : term) (r : ren) :
+  (forall Δ Γ ρ t, F Γ t -> (Δ ⊢ ρ :: Γ) -> F Δ t⟨ρ⟩) ->
+  (Δ ⊢ r :: Γ) ->
+  covered F Γ t ->
+  covered F Δ t⟨r⟩.
+Proof.
+  intros HF Hren Hcov.
+  induction Hcov in Δ, r, Hren |- * ; cbn ; econstructor ; now eauto with typing.
+Qed.
+
+Lemma ren_value (Δ Γ : context) (T : type) (t : term) (r : ren) :
+  value Γ T t ->
+  (Δ ⊢ r :: Γ) ->
+  value Δ T t⟨r⟩.
+Proof.
+  intros Hval Hren.
+  induction T in Γ, Δ, t, r, Hren, Hval |- * ; cbn in *;
+    try solve [intuition eauto using ren_covered with typing].
+  - eapply ren_covered ; eauto.
+    intuition eauto with typing. 
+  - split ; [intuition eauto with typing|].
+    intros b.
+    destruct Hval as [_ Hval].
+    specialize (Hval b) as [u Hu].
+    exists (u⟨r⟩).
+    split ; [|now destruct b ; intuition eauto with typing].
+    change (tProj b t⟨r⟩) with ((tProj b t)⟨r⟩).
+    now apply R_ren.
+  - split ; [intuition eauto with typing|].
+    intros Ξ **.
+    edestruct Hval as [_ [v ]].
+    1: eapply ren_comp_has_type ; cycle -1 ; eassumption.
+    1: eassumption.
+    exists v.
+    now asimpl ; refold.
+  - eapply ren_covered ; tea.
+    intros ?? r' ? Hval' **.
+    destruct Hval' as [|[[a [->]]|[b [->]]]].
+    + left ; eauto with typing.
+    + right ; left.
+      now exists (a⟨r'⟩).
+    + right ; right.
+      now exists b⟨r'⟩.
+Qed.
+
+Lemma ren_red (Δ Γ : context) (T : type) (t : term) (r : ren) :
+  reducible Γ T t ->
+  (Δ ⊢ r :: Γ) ->
+  reducible Δ T t⟨r⟩.
+Proof.
+  intros [u ] ?.
+  exists (u⟨r⟩).
+  split.
+  - now apply R_ren.
+  - now eapply ren_value.
+Qed.
+
+Lemma sem_ren_subst (Ξ Δ Γ : context) (γ : subst) (r : ren) :
+  (Δ ⊩ γ :: Γ) ->
+  (Ξ ⊢ r :: Δ) ->
+  Ξ ⊩ γ >> ren_term r :: Γ.
+Proof.
+  intros Hγ ? i **.
+  cbn.
+  now eapply ren_red.
+Qed.
+
+(** *** Semantic typing of various substitutions *)
+
+Lemma sem_id (Γ : context) : (Γ ⊩ ids :: Γ).
+Proof.
+  intros i ** ; cbn.
+  apply value_red, reflect.
+  eauto with typing.
+Qed.
+
+(** Semantic typing implies reducibility *)
+Corollary sem_red (Γ : context) (A : type) (t : term) : (Γ ⊩ t :: A) -> reducible Γ A t.
+Proof.
+  intros Ht.
+  specialize (Ht Γ ids (sem_id _)).
+  enough (t[ids] = t) as [] by easy.
+  now asimpl.
+Qed.
+
+Lemma sem_Up {Δ Γ : context} {A : type} {γ : subst} : (Δ ⊩ γ :: Γ) -> (Δ,,A) ⊩ ⇑ γ :: (Γ ,, A).
+Proof.
+  intros Hγ [|] T ? ; cbn in * ; refold.
+  - apply value_red, reflect ; eauto with typing.
+  - eapply ren_red ; eauto with typing.
+Qed.
+
+Lemma sem_cons (Δ Γ : context) (A : type) (γ : subst) (t : term) :
+  (Δ ⊩ γ :: Γ) ->
+  reducible Δ A t ->
+  Δ ⊩ t .: γ :: (Γ ,, A).
+Proof.
+  intros Hγ Ht [|] ? Hin ; cbn.
+  - now inversion Hin ; subst.
+  - now apply Hγ.
+Qed.
+
+Lemma sem_one_subst (Γ : context) (A B : type) (a b : term) :
+  (Γ ⊩ a :: A) -> (Γ,,A ⊩ b :: B) -> (Γ ⊩ b[a..] :: B).
+Proof.
+  intros Ha Hb Δ γ Hγ.
+  edestruct (Hb Δ (a[γ] .: γ)) as [v []].
+  - intros [|] ? Hin ; cbn.
+    + inversion Hin ; subst ; clear Hin.
+      now eapply Ha.
+    + apply Hγ, Hin.
+  - exists v.
+    now asimpl ; refold.
+Qed.
+
+(** *** We can push eliminators to the leaves of a cover *)
+
+Lemma proj_cover F Γ t b :
+  covered F Γ t ->
+  exists v, (tProj b t) ⤳* v /\ covered (fun Δ u => exists u', u = tProj b u' /\ F Δ u') Γ v.
+Proof.
+  induction 1 as [? t | ??? s * ? ? (bl'&el&?) ? (br'&er&?) |] ; cbn.
+  - exists (tAbort t).
+    split.
+    1: now rewrite ST_Proj_Abort.
+    now constructor.
+  - exists (tIf s bl' br').
+    split.
+    1: now rewrite ST_Proj_If, el, er.
+    now econstructor.
+  - exists (tProj b t).
+    split ; [easy|].
+    constructor.
+    now eexists.
+Qed.
+
+Lemma app_cover F Γ f t :
+  covered F Γ f ->
+  exists v, (tApp f t) ⤳* v /\
+    covered (fun Δ u => exists u' ρ, (Δ ⊢ ρ :: Γ) /\ u = tApp u' t⟨ρ⟩ /\ F Δ u') Γ v.
+Proof.
+  intros Hcov.
+  induction Hcov as [? e | ??? s * |? f] in t |- * ; cbn.
+  - exists (tAbort e).
+    split.
+    1: now rewrite ST_App_Abort.
+    now constructor.
+  - specialize (IHHcov1 t⟨↑⟩) as (bl'&el&?).
+    specialize (IHHcov2 t⟨↑⟩) as (br'&er&?).
+    eexists (tIf s bl' br').
+    split.
+    1: now rewrite ST_App_If, el, er.
+    econstructor ; tea.
+    all: eapply map_cover ; tea.
+    all: cbn ; intros ?? (u'&ρ&?&[->]).
+    all: exists u', (↑ >> ρ).
+    all: intuition eauto with typing.
+    all: now asimpl.
+  - exists (tApp f t).
+    split ; [easy|].
+    constructor.
+    eexists _, id.
+    intuition eauto with typing.
+    now asimpl.
+Qed.
+
+Lemma abort_cover F Γ t :
+  covered F Γ t ->
+  exists v, (tAbort t) ⤳* v /\ covered (fun Δ u => exists u', u = tAbort u' /\ F Δ u') Γ v.
+Proof.
+  induction 1 as [? t | ??? s * ? ? (bl'&el&?) ? (br'&er&?) |] ; cbn.
+  - exists (tAbort t).
+    split.
+    1: now rewrite ST_Abort_Abort.
+    now constructor.
+  - exists (tIf s bl' br').
+    split.
+    1: now rewrite ST_Abort_If, el, er.
+    now econstructor.
+  - eexists.
+    split ; [easy|].
+    apply cover_ret.
+    now eexists.
+Qed.
+
+Lemma if_cover F Γ s bl br :
+  covered F Γ s ->
+  exists v, (tIf s bl br) ⤳* v /\
+    covered (fun Δ u => exists u' ρ, (Δ ⊢ ρ :: Γ) /\ u = tIf u' bl⟨⇑ ρ⟩ br⟨⇑ ρ⟩ /\ F Δ u') Γ v.
+Proof.
+  intros Hcov.
+  induction Hcov as [? e | ??? s * |? s] in bl, br |- * ; cbn.
+  - exists (tAbort e).
+    split.
+    1: now rewrite ST_If_Abort.
+    now constructor.
+  - specialize (IHHcov1 bl⟨⇑ ↑⟩ br⟨⇑ ↑⟩) as (bl'&el&?).
+    specialize (IHHcov2 bl⟨⇑ ↑⟩ br⟨⇑ ↑⟩) as (br'&er&?).
+    eexists (tIf s bl' br').
+    split.
+    1: now rewrite ST_If_If, el, er.
+    econstructor ; tea.
+    all: eapply map_cover ; tea.
+    all: cbn ; intros ?? (u'&ρ&?&[->]).
+    all: exists u', (↑ >> ρ).
+    all: intuition eauto with typing.
+    all: now rewrite !up_up_ren.
+  - exists (tIf s bl br).
+    split ; [easy|].
+    constructor.
+    eexists _, id.
+    intuition eauto with typing.
+    now rewrite !up_id.
+Qed.
+
+(** *** Covering and reducibility *)
+
+(** A term covered by reducible term reduces to a term covered by values, by
+  reducing all leaves *)
+Lemma covered_red Γ T t :
+  covered (fun Δ u => reducible Δ T u) Γ t ->
+  exists t', t ⤳* t' /\ covered (fun Δ u => value Δ T u) Γ t'.
+Proof.
+  induction 1 as [? t | ??? s * ? ? (bl'&?&?) ? (br'&?&?)|? ? [t']].
+  - exists (tAbort t).
+    split ; [easy|].
+    now constructor.
+  - exists (tIf s bl' br').
+    split ; [now rewrite R_If_cong|].
+    now econstructor.
+  - exists t' ; split ; [easy|].
+    now constructor.
+Qed.
+
+(** A term covered by values is reducible
+  Proven by induction on the type, if it is positive we are essentially done,
+  otherwise we push observations to the leaves thanks to the above lemmas. *)
+Lemma cover_value Γ T t :
+  covered (fun Δ u => value Δ T u) Γ t ->
+  reducible Γ T t.
+Proof.
+  intros Hcov.
+  induction T in Γ, T , t , Hcov |- *.
+  all: try solve [now exists t ; cbn ; eauto using join_cover].
+  - apply value_red ; cbn.
+    split.
+    + eapply run_nf, map_cover ; tea.
+      cbn ; easy.
+    + intros b.
+      eapply proj_cover in Hcov as [t' []] ; cbn in *.
+      eapply red_antired ; tea.
+      edestruct (covered_red Γ (if b then T1 else T2) t') as (t''&?&?).
+      1:{ 
+        eapply map_cover ; [..|eassumption].
+        cbn.
+        now intros ?? (?&->&[_ Hred]).
+      }
+      destruct b ; now eapply red_antired.
+  - apply value_red ; cbn.
+    split.
+    + eapply run_nf, map_cover ; tea.
+      cbn ; easy.
+    + intros Δ u ρ Hρ Hred.
+      eapply ren_covered in Hcov ; tea.
+      2: now eauto using ren_value.
+      apply (app_cover _ _ _ u) in Hcov as [t' []] ; cbn in *.
+      eapply red_antired ; tea.
+      edestruct (covered_red Δ T2 t') as (t''&?&?).
+      1:{ 
+        eapply map_cover ; [..|eassumption].
+        cbn.
+        intros ?? (f&?&?&->&[_ Hred']).
+        replace f with f⟨id⟩ by now asimpl.
+        apply Hred' ; eauto with typing.
+        now eapply ren_red.
+      }
+      now eapply red_antired.
+Qed.
+
+(** Any term covered by reducible terms is reducible *)
+Lemma cover_reducible Γ T t :
+  covered (fun Δ u => reducible Δ T u) Γ t ->
+  reducible Γ T t.
+Proof.
+  intros (?&?&?)%covered_red.
+  eauto using red_antired, cover_value.
+Qed.
+
+(** *** Semantic typing lemmas *)
+
+Lemma sem_Var n Γ T :
+  in_context n Γ T ->
+  Γ ⊩ tVar n :: T.
+Proof.
+  intros Hin Δ γ Hγ.
+  specialize (Hγ _ _ Hin).
+  assumption.
+Qed.
+
+Lemma sem_Star Γ :
+  Γ ⊩ tStar :: TUnit.
+Proof.
+  intros ? ** ; cbn.
+  apply value_red ; cbn.
+  now econstructor.
+Qed.
+
+Lemma sem_App Γ A B f u :
+  (Γ ⊩ f :: TFun A B) ->
+  (Γ ⊩ u :: A) ->
+  Γ ⊩ tApp f u :: B.
+Proof.
+  intros Hf Hu Δ γ Hγ.
+  cbn.
+  destruct (Hf _ γ Hγ) as [f' (Hredf&?&Hf')].
+  destruct (Hu _ γ Hγ) as [u' [Hredu]].
+  cbn in *.
+  apply (red_antired (tApp f' u')).
+  - replace f' with (f'⟨ids⟩) by (now asimpl).
+    apply Hf'.
+    1: now eauto with typing.
+    now apply value_red.
+  - now rewrite Hredf, Hredu.
+Qed.
+
+Lemma sem_Pair Γ A B a b :
+  (Γ ⊩ a :: A) ->
+  (Γ ⊩ b :: B) ->
+  (Γ ⊩ tPair a b :: TProd A B).
+Proof.
+  intros Ha Hb Δ γ Hγ.
+  destruct (Ha _ γ Hγ) as [a' [Hreda]].
+  destruct (Hb _ γ Hγ) as [b' [Hredb]].
+  exists (tPair a' b').
+  split ; [|split] ; cbn.
+  - now rewrite Hreda, Hredb.
+  - auto using reify with typing.
+  - intros [].
+    all: eapply red_antired ; [now apply value_red|].
+    all: now rewrite ?ST_Fst, ?ST_Snd.
+Qed.
+
+Lemma sem_Fst Γ A B t :
+  (Γ ⊩ t :: TProd A B) ->
+  (Γ ⊩ tFst t :: A).
+Proof.
+  intros Ht Δ γ Hγ.
+  specialize (Ht _ _ Hγ) as [t' [Hred [? IH]]] ; cbn in *.
+  apply (red_antired (tFst t')).
+  2: now rewrite Hred.
+  now specialize (IH true).
+Qed.
+
+Lemma sem_Snd Γ A B t :
+  (Γ ⊩ t :: TProd A B) ->
+  (Γ ⊩ tSnd t :: B).
+Proof.
+  intros Ht Δ γ Hγ.
+  specialize (Ht _ _ Hγ) as [t' [Hred [? IH]]] ; cbn in *.
+  apply (red_antired (tSnd t')).
+  2: now rewrite Hred.
+  now specialize (IH false).
+Qed.
+
+Lemma sem_Lam Γ A B t :
+  (Γ ,, A ⊩ t :: B) ->
+  Γ ⊩ tLam t :: TFun A B.
+Proof.
+  intros Ht Δ γ Hγ.
+  cbn ; refold.
+  edestruct (Ht (Δ,,A) (⇑ γ)) as [u [Hred]].
+  1: now eapply sem_Up.
+  exists (tLam u).
+  split ; [now rewrite Hred|].
+  cbn.
+  split.
+  1: now eauto using reify with typing.
+  intros Ξ v ** ; refold.
+  eapply red_antired.
+  2: rewrite ST_Beta_Fun ; reflexivity.
+  edestruct (Ht Ξ) as [v' [Hred']].
+  1:{
+    apply sem_cons ; [|eassumption].
+    now eapply sem_ren_subst.
+  }
+  exists v' ; split ; [|easy].
+  replace (t[_]) with (t[⇑ γ]⟨⇑ ρ⟩[v..]) in Hred'
+    by (substify ; now asimpl).
+  (* confluence *)
+Admitted.
+
+Lemma sem_Abort Γ A t :
+  (Γ ⊩ t :: TEmp) ->
+  (Γ ⊩ tAbort t :: A).
+Proof.
+  intros Ht Δ γ Hγ.
+  specialize (Ht _ _ Hγ) as [t' [Hred Hne]] ; cbn in *.
+  eapply abort_cover in Hne as (t''&Hred'&?).
+  eapply red_antired.
+  2: now rewrite Hred, Hred'.
+  eapply cover_reducible, map_cover ; tea.
+  intros ?? (?&->&?).
+  eapply cover_reducible.
+  now constructor.
+Qed.
+
+Lemma sem_Left Γ A B t :
+  (Γ ⊩ t :: A) ->
+  (Γ ⊩ tLeft t :: TSum A B).
+Proof.
+  intros Ht Δ γ Hγ.
+  specialize (Ht _ _ Hγ) as [t' [Hred Hval]] ; cbn in *.
+  exists (tLeft t').
+  split ; [now rewrite Hred|].
+  constructor.
+  right ; left.
+  now eexists.
+Qed.
+
+Lemma sem_Right Γ A B t :
+  (Γ ⊩ t :: B) ->
+  (Γ ⊩ tRight t :: TSum A B).
+Proof.
+  intros Ht Δ γ Hγ.
+  specialize (Ht _ _ Hγ) as [t' [Hred Hval]] ; cbn in *.
+  exists (tRight t').
+  split ; [now rewrite Hred|].
+  constructor.
+  right ; right.
+  now eexists.
+Qed.
+
+Lemma sem_If Γ A B T s bl br :
+  (Γ ⊩ s :: TSum A B) ->
+  (Γ,,A ⊩ bl :: T) ->
+  (Γ,,B ⊩ br :: T) ->
+  (Γ ⊩ tIf s bl br :: T).
+Proof.
+  intros Hs Hl Hr Δ γ Hγ.
+  specialize (Hs _ _ Hγ) as [s' [Hred Hne]] ; cbn in *.
+  eapply if_cover in Hne as (t''&Hred'&?).
+  eapply red_antired.
+  2: now rewrite Hred, Hred'.
+  eapply cover_reducible, map_cover ; tea.
+  intros Δ' ? (?&ρ&?&->&Hval).
+  eapply cover_reducible.
+  constructor.
+  destruct Hval as [| [(a&->&?)|(b&->&?)]].
+  - eapply cover_reducible.
+    rewrite !up_up_subst_ren.
+    econstructor ; tea.
+    all: constructor.
+    + now eapply Hl, sem_Up, sem_ren_subst.
+    + now eapply Hr, sem_Up, sem_ren_subst.
+  - eapply red_antired.
+    2: now rewrite ST_Left.
+    replace (_[_..]) with (bl[a .: (γ >> ren_term ρ)]).
+    2:{ substify ; asimpl ; refold.
+        apply subst_term_morphism ; [|easy].
+        intros [|] ; cbn ; [easy|].
+        apply subst_term_morphism ; [|easy].
+        now intros [|].
+    }
+    eapply Hl, sem_cons.
+    2: now apply value_red.
+    now eapply sem_ren_subst.
+  - eapply red_antired.
+    2: now rewrite ST_Right.
+    replace (_[_..]) with (br[b .: (γ >> ren_term ρ)]).
+    2:{ substify ; asimpl ; refold.
+        apply subst_term_morphism ; [|easy].
+        intros [|] ; cbn ; [easy|].
+        apply subst_term_morphism ; [|easy].
+        now intros [|].
+    }
+    eapply Hr, sem_cons.
+    2: now apply value_red.
+    now eapply sem_ren_subst.
+Qed.
+
+Theorem fundamental Γ T (t : term) :
+  (Γ ⊢ t :: T) ->
+  (Γ ⊩ t :: T).
+Proof.
+  intros Hty.
+  induction Hty.
+  - now apply sem_Var.
+  - now apply sem_Star.
+  - now apply sem_Lam.
+  - now eapply sem_App.
+  - now eapply sem_Pair.
+  - now eapply sem_Fst.
+  - now eapply sem_Snd.
+  - now eapply sem_Abort.
+  - now eapply sem_Left.
+  - now eapply sem_Right.
+  - now eapply sem_If.
+Qed.
+
+Corollary normalisation Γ T (t : term) :
+  (Γ ⊢ t :: T) ->
+  exists u, (t ⤳* u) /\ (Γ ⊢ u ◃ T).
+Proof.
+  intros []%fundamental%sem_red.
+  eexists ; split ; intuition eauto using reify.
+Qed.
