code/theories/Utils.v
@@ -44,6 +44,7 @@ Infix "=1" := (pointwise_relation _ Logic.eq) (at level 70).
 (** ** Tactics *)
 
 Hint Constructors eq : core.
+Hint Extern 10 => reflexivity : core.
 
 (* To use in intro patterns, similar to SSReflects' /dup view *)
 Definition dup {A : Type} : A -> A * A := fun x => (x,x).
